refactor: reorganize types & type refs

LeanPy/Data/Object/ObjectType.lean
@@ -3,11 +3,11 @@ Copyright (c) 2025 Mac Malone. All rights reserved.
 Released under the Apache 2.0 license as described in the file LICENSE.
 Authors: Mac Malone
 -/
-import LeanPy.Data.Object.Type
+import LeanPy.Data.Object.InitTypeRef
 
 namespace LeanPy
 
-def objectTypeDoc : String := "\
+def objectType.doc : String := "\
   The base class of the class hierarchy.\n\
   \n\
   When called, it accepts no arguments and returns a new featureless\n\
@@ -16,8 +16,8 @@ def objectTypeDoc : String := "\
 
 @[reducible] def objectType : PyType where
   name := "object"
-  doc? := some objectTypeDoc
+  doc? := some objectType.doc
 
-initialize objectTypeRef' : DTypeRef objectType ← mkDTypeRef _
+initialize objectTypeRef.init : InitTypeRef objectType ← initTypeRef
 
-abbrev objectTypeRef : TypeRef := objectTypeRef'.toTypeRef
+abbrev objectTypeRef : TypeRef := objectTypeRef.init.toTypeRef
