LeanPy/Data/Object/Type.lean
@@ -8,9 +8,19 @@ import LeanPy.Data.Object.Data
 
 namespace LeanPy
 
-/-! ## Object Type -/
+/-! ## Raw Object Prop -/
 
-/-- A Python type. -/
+def ObjectProp.Raw :=
+  (id : ObjectId) → (data : ObjectData) → Prop
+
+@[simp] def ObjectProp.Raw.Any : ObjectProp.Raw :=
+  fun _ _ => True
+
+instance : Nonempty ObjectProp.Raw := ⟨.Any⟩
+
+/-! ## Type -/
+
+/-- A raw Python type. -/
 -- The `Py` prefix to avoids a clash with the Lean `Type` keyword.
 structure PyType where
   /-- The type's name -/
@@ -50,212 +60,12 @@ structure PyType where
   This can be an over-approximation. That is, it may hold for objects
   which are not objects of this type.
   -/
-  IsValidObject (id : ObjectId) (data : ObjectData) : Prop := True
+  IsValidObject : ObjectProp.Raw := .Any
   deriving Nonempty
 
-namespace PyType
+/-! ## Raw Type Ref -/
 
-/-- The type's method resolution order. -/
-@[inline] def mro (self : PyType) : List PyType :=
-  self :: match self with
-    | {base? := none, ..} => []
-    | {base? := some base, ..} => mro base.data
+/-- A `TypeRef` as represented recursively in `PyType`. -/
+abbrev RawTypeRef := FrozenRef PyType
 
-@[inline] def baseMro (self : PyType) : List PyType :=
-  match self with
-  | {base? := none, ..} => []
-  | {base? := some base, ..} => mro base.data
-
-theorem mro_def : mro self = self :: baseMro self := by
-  unfold mro baseMro; rfl
-
-theorem mem_mro_iff : ty ∈ mro self ↔ ty = self ∨ ty ∈ baseMro self := by
-  simp [mro_def]
-
-@[simp] theorem self_mem_mro : self ∈ mro self := by
-  simp [mro_def]
-
-@[simp] theorem baseMro_subset_mro : baseMro self ⊆ mro self := by
-  simp [mro_def]
-
-theorem mem_mro_of_mem_baseMro : ty ∈ baseMro self → ty ∈ mro self :=
-  List.subset_def.mp baseMro_subset_mro
-
-private theorem mem_mro_trans :
-  ty₁ ∈ mro ty₂ → ty₂ ∈ mro self → ty₁ ∈ mro self
-:= by
-  revert ty₂
-  let {base?, ..} := self
-  cases base? with
-  | none =>
-    intro ty₂ h₁
-    simp only [mro, List.mem_cons, List.not_mem_nil, or_false]
-    intro h₂
-    simpa [h₂, mro] using h₁
-  | some base =>
-    intro ty₂ h₁
-    simp only [mro, List.mem_cons]
-    intro h₂
-    cases h₂ with
-    | inl h₂ => simpa [h₂, mro] using h₁
-    | inr h₂ => exact Or.inr <| mem_mro_trans h₁ h₂
-
-def IsSubtype (self other : PyType) : Prop :=
-  other ∈ self.mro
-
-instance : HasSubset PyType := ⟨PyType.IsSubtype⟩
-
-theorem subset_iff_mem_mro : a ⊆ b ↔ b ∈ mro a := Iff.rfl
-
-@[simp] theorem subset_rfl {self : PyType} : self ⊆ self :=  self_mem_mro
-
-theorem subset_trans {a b c : PyType} : a ⊆ b → b ⊆ c → a ⊆ c  := by
-  simp only [subset_iff_mem_mro]
-  exact fun h₁ h₂ => mem_mro_trans h₂ h₁
-
-end PyType
-
-/-! ## Object Type Ref -/
-
-abbrev TypeRef := FrozenRef PyType
-
-noncomputable instance : SizeOf TypeRef :=
-  inferInstanceAs (SizeOf (FrozenRef PyType))
-
-namespace TypeRef
-
-instance : TypeName TypeRef := unsafe (.mk _ ``TypeRef)
-
-/-- The type's method resolution order. -/
-@[inline] def mro (self : TypeRef) : List TypeRef :=
-  self :: go self.data
-where go self :=
-  match self with
-  | {base? := none, ..} => []
-  | {base? := some base, ..} => mro base
-
-@[inline] def baseMro (self : TypeRef) : List TypeRef :=
-  match self.data with
-  | {base? := none, ..} => []
-  | {base? := some base, ..} => mro base
-
-instance : SizeOf TypeRef := ⟨(·.baseMro.length)⟩
-
-@[simp] theorem sizeOf_def {self : TypeRef} :
-  sizeOf self = self.baseMro.length
-:= rfl
-
-theorem mro_def : mro self = self :: baseMro self := by
-  unfold mro baseMro mro.go; simp
-
-@[simp] theorem length_mro : (mro self).length = self.baseMro.length + 1 := by
-  simp [mro_def]
-
-theorem mem_mro_iff : ty ∈ mro self ↔ ty = self ∨ ty ∈ baseMro self := by
-  simp [mro_def]
-
-@[simp] theorem self_mem_mro : self ∈ mro self := by
-  simp [mro_def]
-
-@[simp] theorem baseMro_subset_mro : baseMro self ⊆ mro self := by
-  simp [mro_def]
-
-private theorem sup_mem_sub :
-  sup ∈ mro sub → ∀ {ty}, ty ∈ mro sup → ty ∈ mro sub
-:= by
-  simp only [mem_mro_iff]
-  match h_sub:sub.data with
-  | {base? := none, ..} =>
-    simp only [baseMro, h_sub, List.not_mem_nil, or_false]
-    intro sup_eq_sub
-    intro ty
-    simp [sup_eq_sub, h_sub]
-  | {base? := some base, ..} =>
-    have sub_baseMro : sub.baseMro = mro base := by
-      simp [h_sub, baseMro]
-    simp only [sub_baseMro]
-    intro h ty
-    cases h with
-    | inl sup_eq_sub =>
-      simp [sup_eq_sub, sub_baseMro]
-    | inr sup_mem_mro_base =>
-      simp only [← mem_mro_iff]
-      intro ty_mem
-      exact Or.inr <| sup_mem_sub sup_mem_mro_base ty_mem
-termination_by sub
-decreasing_by simp [sub_baseMro]
-
-def Subtype (self other : TypeRef) : Prop :=
-  other ∈ self.mro
-
-instance : HasSubset TypeRef := ⟨TypeRef.Subtype⟩
-
-theorem subset_iff_mem_mro : a ⊆ b ↔ b ∈ mro a := Iff.rfl
-
-theorem subset_iff_eq_or_mem_baseMro : a ⊆ b ↔ (a = b ∨ b ∈ baseMro a) := by
-  grind [subset_iff_mem_mro, mro_def]
-
-@[simp] theorem Subtype.rfl {self : TypeRef} : self ⊆ self := self_mem_mro
-
-@[simp] theorem Subtype.refl (self : TypeRef) : self ⊆ self := self_mem_mro
-
-theorem Subtype.trans {a b c : TypeRef} : a ⊆ b → b ⊆ c → a ⊆ c  := by
-  simp only [subset_iff_mem_mro]
-  exact fun h₁ h₂ => sup_mem_sub h₁ h₂
-
-instance : Trans (Subset : TypeRef → TypeRef → Prop) Subset Subset :=
-  ⟨Subtype.trans⟩
-
-@[inherit_doc PyType.name]
-abbrev name (self : TypeRef) : String :=
-  self.data.name
-
-@[simp, inherit_doc PyType.isTypeSubclass]
-abbrev isTypeSubclass (self : TypeRef) : Bool :=
-  self.data.isTypeSubclass
-
-@[simp, inherit_doc PyType.isIntSubclass]
-abbrev isIntSubclass (self : TypeRef) : Bool :=
-  self.data.isIntSubclass
-
-@[simp, inherit_doc PyType.isStrSubclass]
-abbrev isStrSubclass (self : TypeRef) : Bool :=
-  self.data.isStrSubclass
-
-@[simp, inherit_doc PyType.IsValidObject]
-abbrev IsValidObject (self : TypeRef) (id : ObjectId) (data : ObjectData) : Prop :=
-  self.data.IsValidObject id data
-
-end TypeRef
-
-structure DTypeRef (ty : PyType) extends NonScalarRef PyType where
-  data_eq : toNonScalarRef.data = ty
-
-namespace DTypeRef
-
-attribute [simp] data_eq
-
-instance : Nonempty (DTypeRef ty) := ⟨⟨.null ty, rfl⟩⟩
-
-@[inline] def toTypeRef (self : DTypeRef ty) : TypeRef :=
-  self.toFrozenRef.cast self.data_eq
-
-@[simp] theorem isNonScalar_addr_toTypeRef {self : DTypeRef ty} :
-  self.toTypeRef.addr % 2 = 0
-:= self.addr_mod_two
-
-end DTypeRef
-
-instance : CoeOut (DTypeRef ty) TypeRef :=
-  ⟨DTypeRef.toTypeRef⟩
-
-@[inline] private unsafe def mkTypeRefImpl
-  (ty : PyType) : BaseIO (DTypeRef ty)
-:= pure (unsafeCast ty)
-
-@[implemented_by mkTypeRefImpl]
-opaque mkDTypeRef (ty : PyType) : BaseIO (DTypeRef ty) :=
-  pure ⟨NonScalarRef.null ty, NonScalarRef.data_null⟩
-
-@[inline] def mkTypeRef (ty : PyType) : BaseIO TypeRef := do
-  (·.toTypeRef) <$> mkDTypeRef ty
+instance : TypeName RawTypeRef := unsafe (.mk _ ``RawTypeRef)
