LeanPy/Data/Object/InitTypeRef.lean
@@ -1,0 +1,50 @@
+/-
+Copyright (c) 2025 Mac Malone. All rights reserved.
+Released under the Apache 2.0 license as described in the file LICENSE.
+Authors: Mac Malone
+-/
+import LeanPy.Data.Object.TypeRef
+
+namespace LeanPy
+
+/-! ## Fixed Type Ref -/
+
+/--
+A reference to a statically known `PyType`.
+
+This is used to initialize types.
+-/
+structure InitTypeRef (ty : PyType) extends NonScalarRef PyType where
+  data_eq : toNonScalarRef.data = ty
+
+namespace InitTypeRef
+
+attribute [simp] InitTypeRef.data_eq
+
+instance : Nonempty (InitTypeRef ty) := ⟨⟨.null ty, rfl⟩⟩
+
+@[inline] def toTypeRef (self : InitTypeRef ty) : TypeRef :=
+  ⟨self.toFrozenRef.cast self.data_eq⟩
+
+@[simp] theorem isNonScalar_addr_toRawTypeRef {self : InitTypeRef ty} :
+  self.toTypeRef.addr % 2 = 0
+:= self.addr_mod_two
+
+instance : CoeOut (InitTypeRef ty) TypeRef :=
+  ⟨InitTypeRef.toTypeRef⟩
+
+end InitTypeRef
+
+@[inline] private unsafe def initTypeRefImpl
+  (ty : PyType) : BaseIO (InitTypeRef ty)
+:= pure (unsafeCast ty)
+
+@[implemented_by initTypeRefImpl]
+opaque initTypeRef {ty : PyType} : BaseIO (InitTypeRef ty) :=
+  pure ⟨NonScalarRef.null ty, NonScalarRef.data_null⟩
+
+@[inline] def mkInitTypeRef (ty : PyType) : BaseIO (InitTypeRef ty) := do
+  initTypeRef
+
+@[inline] def mkTypeRef (ty : PyType) : BaseIO TypeRef := do
+  (·.toTypeRef) <$> mkInitTypeRef ty
