LeanPy/Data/Object/LawfulTypeRef.lean
@@ -1,0 +1,87 @@
+/-
+Copyright (c) 2025 Mac Malone. All rights reserved.
+Released under the Apache 2.0 license as described in the file LICENSE.
+Authors: Mac Malone
+-/
+import LeanPy.Data.Object.TypeRef
+import LeanPy.Data.Object.ObjectTypes2
+
+namespace LeanPy
+
+/-! ## LawfulTypeRef -/
+
+class LawfulTypeRef (self : TypeRef) : Prop where
+  isNonScalar_addr : self.addr % 2 = 0 := by simp
+  subset_objectType : self ⊆ objectTypeRef := by
+    simp [TypeRef.subset_iff_mem_mro, TypeRef.mro_eq_cons_baseMro, TypeRef.eq_iff]
+  isTypeSubclass_iff_subset :
+    self.isTypeSubclass ↔ self ⊆ typeTypeRef := by
+      simp [TypeRef.subset_iff_mem_mro, TypeRef.mro_eq_cons_baseMro, TypeRef.eq_iff]
+  isIntSubclass_iff_subset :
+    self.isIntSubclass ↔ self ⊆ intTypeRef := by
+      simp [TypeRef.subset_iff_mem_mro, TypeRef.mro_eq_cons_baseMro, TypeRef.eq_iff]
+  isStrSubclass_iff_subset :
+    self.isStrSubclass ↔ self ⊆ strTypeRef := by
+      simp [TypeRef.subset_iff_mem_mro, TypeRef.mro_eq_cons_baseMro, TypeRef.eq_iff]
+  isValidObject_mro {id data} :
+    self.IsValidObject id data → ∀ {ty}, self ⊆ ty → ty.IsValidObject id data
+  := by simp_all [TypeRef.subset_iff_mem_mro, TypeRef.mro_eq_cons_baseMro]
+
+namespace TypeRef
+
+export LawfulTypeRef (
+  isNonScalar_addr subset_objectType
+  isTypeSubclass_iff_subset isIntSubclass_iff_subset isStrSubclass_iff_subset
+  isValidObject_mro
+)
+
+@[inline] def toNonScalarRef (self : TypeRef) [LawfulTypeRef self] : NonScalarRef PyType :=
+  NonScalarRef.mk self.toRawTypeRef isNonScalar_addr
+
+abbrev id (self : TypeRef) [LawfulTypeRef self] : ObjectId :=
+  self.toNonScalarRef.id
+
+end TypeRef
+
+@[simp] theorem data_objectTypeRef : objectTypeRef.data = objectType := rfl
+
+@[simp] theorem mro_objectTypeRef :
+  objectTypeRef.baseMro = []
+:= rfl
+
+@[simp] theorem data_typeTypeRef : typeTypeRef.data = typeType := rfl
+
+@[simp] theorem baseMro_typeTypeRef :
+  typeTypeRef.baseMro = [objectTypeRef]
+:= rfl
+
+@[simp] theorem data_noneTypeRef : noneTypeRef.data = noneType := rfl
+
+@[simp] theorem baseMro_noneTypeRef :
+  noneTypeRef.baseMro = [objectTypeRef]
+:= rfl
+
+@[simp] theorem data_strTypeRef : strTypeRef.data = strType := rfl
+
+@[simp] theorem baseMro_strTypeRef :
+  strTypeRef.baseMro = [objectTypeRef]
+:= rfl
+
+@[simp] theorem data_intTypeRef : intTypeRef.data = intType := rfl
+
+@[simp] theorem baseMro_intTypeRef :
+  intTypeRef.baseMro = [objectTypeRef]
+:= rfl
+
+@[simp] theorem data_boolTypeRef : boolTypeRef.data = boolType := rfl
+
+@[simp] theorem baseMro_boolTypeRef :
+  boolTypeRef.baseMro = [intTypeRef, objectTypeRef]
+:= rfl
+
+instance : LawfulTypeRef objectTypeRef where
+instance : LawfulTypeRef typeTypeRef where
+instance : LawfulTypeRef noneTypeRef where
+instance : LawfulTypeRef strTypeRef where
+instance : LawfulTypeRef intTypeRef where
+instance : LawfulTypeRef boolTypeRef where
