tests/api.lean
@@ -6,10 +6,10 @@ open LeanPy
 #guard_msgs in #eval return (← mkObjectObject).beq (← mkObjectObject)
 
 /-- info: true -/
-#guard_msgs in #eval (intTypeRef' : Object).asObject.beq (intTypeRef' : Object)
+#guard_msgs in #eval (intTypeRef : Object).asObject.beq (intTypeRef : Object)
 
 /-- info: false -/
-#guard_msgs in #eval (intTypeRef' : Object).asObject.beq (boolTypeRef' : Object)
+#guard_msgs in #eval (intTypeRef : Object).asObject.beq (boolTypeRef : Object)
 
 /-- info: false -/
-#guard_msgs in #eval (intTypeRef' : Object).asObject.beq (0 : Object)
+#guard_msgs in #eval (intTypeRef : Object).asObject.beq (0 : Object)
